ntor/Security.ec
@@ -155,15 +155,15 @@ module (Red_ROM2 (D : A_GAKE) (O1 : ROSc.I1.RO) : ROSc.I2.RO_Distinguisher) (O2 
     ]
 
     proc c_test [
-      ^match#Some.^match#Accepted.^if.^ks<$ -
-      ^match#Some.^match#Accepted.^if.^if -
-      ^match#Some.^match#Accepted.^if.^k<- ~ {ks <@ O2.get(x); k <- Some ks;}
+      ^if.^match#Some.^match#Accepted.^if.^ks<$ -
+      ^if.^match#Some.^match#Accepted.^if.^if -
+      ^if.^match#Some.^match#Accepted.^if.^k<- ~ {ks <@ O2.get(x); k <- Some ks;}
     ]
 
     proc s_test [
-      ^match#Some.^match#Accepted.^if.^ks<$ -
-      ^match#Some.^match#Accepted.^if.^if -
-      ^match#Some.^match#Accepted.^if.^k<- ~ {ks <@ O2.get(x); k <- Some ks;}
+      ^if.^match#Some.^match#Accepted.^if.^ks<$ -
+      ^if.^match#Some.^match#Accepted.^if.^if -
+      ^if.^match#Some.^match#Accepted.^if.^k<- ~ {ks <@ O2.get(x); k <- Some ks;}
     ]  
   }
 
@@ -180,7 +180,7 @@ module (Red_ROM2 (D : A_GAKE) (O1 : ROSc.I1.RO) : ROSc.I2.RO_Distinguisher) (O2 
 (* ------------------------------------------------------------------------------------------ *)
 section.
 
-declare module A <: A_GAKE {-GAKE0, -Game0, -Game1, -Game2, -ROc.IdealAll.RO, -RO, -FRO, -ROSc.I1.RO, -ROSc.I2.RO, -ROSc.I1.FRO, -ROSc.I2.FRO, -Red_Coll, -BB.Sample, -Red_ROM, -Red_ROM2 }.
+declare module A <: A_GAKE {-GAKE0, -Game0, -Game1, -Game2, -Game3, -Game4, -ROc.IdealAll.RO, -RO, -FRO, -ROSc.I1.RO, -ROSc.I2.RO, -ROSc.I1.FRO, -ROSc.I2.FRO, -Red_Coll, -BB.Sample, -Red_ROM, -Red_ROM2 }.
 
 declare axiom A_ll (G <: GAKE_out{-A}):
   islossless G.h =>
@@ -201,12 +201,358 @@ declare axiom A_ll (G <: GAKE_out{-A}):
 declare axiom A_bounded_qs: forall (G <: GAKE_out{-A}), hoare[A(Counter(G)).run: Counter.cis = 0 /\ Counter.cm1 = 0 /\ Counter.cm2 = 0 ==> Counter.cis <= q_is /\ Counter.cm1 <= q_m1 /\ Counter.cm2 <= q_m2].
 
 
+(* ------------------------------------------------------------------------------------------ *)
+(* Step 4: Introducing event of collision between test query and queries made to the RO by the adversary. *)
+lemma Step4 &m :
+  Pr[E_GAKE(Game2, A).run() @ &m : res] = Pr[E_GAKE(Game3, A).run() @ &m : res].
+proof. 
+byequiv => //; sim.
+qed. 
+
+
+(* ------------------------------------------------------------------------------------------ *)
+(* Step 5a:  Removing RO for storing keys *)
+lemma Step5a &m :
+  Pr[E_GAKE(Game3, A).run() @ &m : res /\ (oget Game3.tq \notin Game3.hq) ]
+  =
+  Pr[E_GAKE(Game4, A).run() @ &m : res /\ (oget Game4.tq \notin Game4.hq)].
+proof. 
+byequiv => //. 
+proc; inline.
+call (: ={servers, c_smap, s_smap, tested, kp_set, bad, hm, h1m, h2m, hq, tq}(Game3, Game4)); try sim />. (* TODO : add the badq event *)
+
+- proc.
+  sp; if => //.
+  sp; match = => // st.
+  match = => // st' t' k' ir'.
+  if => //.
+  rcondt{1} ^if. 
+  - auto => />. admit. (* TODO: Invariant! *)
+  auto => /> &1 &2 *. rewrite get_setE => /=.
+  admit. (* TODO: h2m not equal! *)
+
+ - proc.
+  sp; if => //.
+  sp; match = => // st.
+  match = => // st' t' k' ir'.
+  if => //.
+  rcondt{1} ^if. 
+  - auto => />. admit. (* TODO: Invariant! *)
+  auto => /> &1 &2 *. rewrite get_setE => /=.
+  admit. (* TODO: h2m not equal! *)
+
+qed. 
+
+
+(* ------------------------------------------------------------------------------------------ *)
+(* Step 6a: Equivalence to the ideal Game  *)
+lemma Step6a &m :
+  Pr[E_GAKE(Game4, A).run() @ &m : res /\ (oget Game4.tq \notin Game4.hq) ]
+  =
+  Pr[E_GAKE(GAKE1(NTOR_S(RO), NTOR_C(RO), RO), A).run() @ &m : res].
+proof. 
+byequiv => //.
+proc; inline.
+call (: ={servers, c_smap, s_smap, tested}(Game4, GAKEb) /\ RO.m{2} = Game4.hm{1}); try sim />; admit.
+
+qed.
+
+
+(* ------------------------------------------------------------------------------------------ *)
+(* Step 5b: Starting the crypto part  *)
+
+
+
+
+(* ------------------------------------------------------------------------------------------ *)
+(* Step 0: Inlining everything. *)
+lemma Step0 &m :
+  Pr[E_GAKE(GAKE0(NTOR_S(RO), NTOR_C(RO), RO), A).run() @ &m : res] = Pr[E_GAKE(Game0, A).run() @ &m : res].
+proof. 
+byequiv => //.
+proc; inline.
+call (: ={servers, c_smap, s_smap, tested}(GAKEb, Game0) /\ RO.m{1} = Game0.hm{2}); try sim />.
+
+- proc; inline; auto; if => //; auto => /#.
+
+- proc; inline. 
+  sp; if => //.
+  sp; match = => // [|st]; 1:by auto.
+  by match = => // st' pt' ir'; auto.
+
+- proc; inline.
+  sp; match = => // sk.
+  match = => //.
+  match Some {1} 4.
+  + by auto=> /> _ _ _ _; exists (b{m0}, sk, None).
+  match Some {1} ^match=> //; 1: by auto=> /> /#.
+  by auto => />.
+
+- proc; inline; auto=> />.
+  sp; match = => //; 1: auto.
+  by match = => //; 1: auto.
+qed.
+
+(* ------------------------------------------------------------------------------------------ *)
+(* Step 1: Remove collisions in ephemeral and long-term keys. *)
+lemma Step1 &m: `| Pr[E_GAKE(Game0, A).run() @ &m : res] - Pr[E_GAKE(Game1, A).run() @ &m : res] | <= Pr[E_GAKE(Game0, A).run() @ &m : Game0.bad].
+proof.
+rewrite StdOrder.RealOrder.distrC.
+byequiv (: _ ==> _) : Game1.bad => //; first last.
++ by rewrite eq_iff.
+symmetry; proc; inline*.
+call (: Game1.bad
+      , ={servers, c_smap, s_smap, tested, kp_set, hm, bad}(Game0, Game1)
+      , ={bad}(Game0, Game1)) => //; try sim />.
+
+- exact A_ll.
+
+- move => &2 bad; proc; auto => />. 
+  by rewrite weight_dprod dkey_ll dtag_ll.
+- move => &1; proc; auto.
+  by rewrite weight_dprod dkey_ll dtag_ll.
+
+- proc.
+  if => //.
+  seq 1 1: (#pre /\ ={kp}); 1: by auto.
+  by sp 0 1; if{2}; auto => />.
+- move => &2 bad.
+  proc; if; auto.
+  rewrite dkp_ll //=. smt().
+- move => &1. 
+  proc; if => //. 
+  rcondf ^if; auto => />.
+  by rewrite dkp_ll.
+
+- move => &2 bad.
+  proc; auto => />.
+- move => &1. 
+  proc; auto => />. 
+
+- proc.
+  sp; if => //.
+  sp; match = => //. 
+  + seq 1 1: (#pre /\ ={kp}); 1: by auto.
+    by sp 0 1; if{2}; auto => />.
+  move => st. 
+  match = => //.
+  move => st' pr' ir'.
+  auto => />.
+- move => &2 bad.
+  proc; sp; if => //; sp. 
+  match; auto => />.
+  + rewrite dkp_ll. smt().
+  by smt().
+- move => &1. 
+  proc; sp; if => //. 
+  sp; match; auto => />.
+  + by rewrite dkp_ll.
+  by smt().
+
+- proc; inline.
+  sp; match = => //. 
+  move => sk.
+  match = => //.
+  + seq 1 1: (#pre /\ ={kp}); 1: by auto.
+  sp 0 1; if{2}.
+  + by auto => />. 
+  auto.
+- move => &2 bad.
+  proc; inline*; sp; match; auto => />.
+  match; auto => />.
+  rewrite dkp_ll weight_dprod dkey_ll dtag_ll. 
+  by smt().
+- move => &1. 
+  proc; sp; match; auto => />.
+  match; 2: by auto => />. 
+  rcondf ^if; 1: by auto => />. 
+  auto => />.
+  by rewrite dkp_ll.
+
+- move => &2 bad.
+  proc; inline.
+  sp; match; auto. 
+  match; auto => />.
+  by rewrite weight_dprod dkey_ll dtag_ll.
+- move => &1.
+  proc; inline*; auto => />.
+  sp; match; auto.
+  match; auto.
+  by rewrite weight_dprod dkey_ll dtag_ll.
+
+- move => &2 bad.
+  proc; sp; match; 1: by auto. 
+  match; auto => />.
+- move => &1.
+  proc; sp; match; 1: by auto. 
+  match; auto => />.
+
+- move => &2 bad.
+  proc; sp; match; 1: by auto. 
+  match; auto => />.
+- move => &1.
+  proc; sp; match; 1: by auto. 
+  match; auto => />.
+
+- move => &2 bad.
+  proc; sp; match; 1: by auto. 
+  match; auto => />.
+- move => &1.
+  proc; sp; match; 1: by auto. 
+  match; auto => />.
+
+- move => &2 bad.
+  proc; sp; match; 1: by auto. 
+  match; auto => />.
+- move => &1.
+  proc; sp; match; 1: by auto. 
+  match; auto => />.
+
+- move => &2 bad.
+  proc; sp; match; 1: by auto. 
+  match; auto => />.
+- move => &1.
+  proc; sp; match; 1: by auto. 
+  match; auto => />.
+
+- move => &2 bad.
+  proc; sp; if => //. sp. admit. (*match. 1: by auto. 
+  match; auto => />.*)
+- move => &1.
+  proc; sp; if => //. sp. admit. (*match; 1: by auto. 
+  match; auto => />.*)
+
+- move => &2 bad.
+  proc; sp; if => //. sp. admit. (*match. 1: by auto. 
+  match; auto => />.*)
+- move => &1.
+  proc; sp; if => //. sp. admit. (*match; 1: by auto. 
+  match; auto => />.*)
+
+auto => />.
+move => rl rr al bl csl hml kpl ssl sl tl ar br csr hmr kpr ssr sr tr. 
+by case : (!br) => />.
+qed.
+
+
+(* ------------------------------------------------------------------------------------------ *)
+(* Step 1b: Bound the bad event. *)
+lemma Step1b &m: Pr[E_GAKE(Game0, A).run() @ &m : Game0.bad] <= ((q_is + q_m1 + q_m2) ^ 2)%r * mu1 dkp (mode dkp).
+proof.
+apply (StdOrder.RealOrder.ler_trans Pr[BB.Exp(BB.Sample, Red_Coll(A)).main() @ &m : ! uniq BB.Sample.l]); first last.
++ apply (BB.pr_collision_q2 (Red_Coll(A))).
+  + move => S S_ll.
+    islossless.
+    apply (A_ll (Counter(Red_Coll_O_AKE(S)))); islossless.
+    + match; 1: auto; islossless.
+      match; auto.
+    + match; auto. 
+      by sp; match; auto; islossless.
+    + match => //.
+      by sp; match; auto; islossless.
+    + match => //; islossless.
+      by match; islossless.
+    + by match; 1: auto; match; islossless.
+    + by match; 1: auto; match; islossless.
+    + by match; 1: auto; match; islossless.
+    + by match; 1: auto; match; islossless.
+    + by match; 1: auto; match; islossless.
+    + by match; 1: auto; match; islossless.
+  proc; inline.
+  sp.
+  conseq (: _ ==> size BB.Sample.l <= Counter.cis + Counter.cm1 + Counter.cm2) (: Counter.cis = 0 /\ Counter.cm1 = 0 /\ Counter.cm2 = 0 ==> Counter.cis <= q_is /\ Counter.cm1 <= q_m1 /\ Counter.cm2 <= q_m2)=> //.
+  + smt().
+  + by call (A_bounded_qs (Red_Coll_O_AKE(BB.Sample))).
+  call (: size BB.Sample.l <= Counter.cis + Counter.cm1 + Counter.cm2) => //.
+  + by proc; auto.
+  + by proc; inline; sp; if => //; auto => /#.
+  + by proc; auto.
+  + proc; inline; sp; if => //; 2: auto => /#.
+    by sp; match; auto => /#.
+  + proc; inline; sp; match; 1: auto => /#.
+    case ((Red_Coll_O_AKE.s_smap.[b, j]) = None).
+    + by match None ^match; auto => /#.
+    by match Some ^match; auto => /#.
+  + by proc; inline; sp; match; 1: auto; match; auto => /#.
+  + by proc; sp; match; 1: auto; match; auto => /#.
+  + by proc; sp; match; 1: auto; match; auto => /#.
+  + by proc; sp; match; 1: auto; match; auto => /#.
+  + by proc; sp; match; 1: auto; match; auto => /#.
+  + by proc; sp; match; 1: auto; match; auto => /#.
+  + admit.
+  + admit.
+  auto => /#.
+byequiv => //.
+proc. inline.
+call (:
+ ={hm, servers, c_smap, s_smap, tested, kp_set, bad}(Game0, Red_Coll_O_AKE(BB.Sample))
+ /\ (Game0.bad{1} => !uniq BB.Sample.l{2})
+ /\ (forall kp, kp \in Game0.kp_set{1} => kp \in BB.Sample.l{2})
+) => //; try sim />.
++ proc; inline; sp 0 2; if => //; auto => />. 
+  smt(mem_set in_fsetU1).
++ proc; inline; sp 2 4; if => //; auto.
+  sp; match = => // [|st].
+  + auto => />.
+    smt(mem_set in_fsetU1).
+  match = => // st' pt ir. 
+  auto => />.
++ proc; inline; sp 2 4; match = => // [|st]; 1: auto.
+  match = => // [|st']; 2: auto.
+  auto => />.
+  smt(mem_set in_fsetU1).
+auto => />.
+smt(in_fset0).
+qed.
+
+
+(* ------------------------------------------------------------------------------------------ *)
+(* Step 2: Splitting the random oracle. *)
+local clone import DProd.ProdSampling with
+  type t1 <- tag,
+  type t2 <- key
+proof *.
+
+lemma Step2 &m: Pr[E_GAKE(Game1, A).run() @ &m : res] = Pr[ROc.IdealAll.MainD(Red_ROM(A), ROSc.RO_Pair(ROSc.I1.RO,ROSc.I2.RO)).distinguish() @ &m : res].
+proof.
+byequiv (: ={glob A, glob Red_ROM} ==> _)  => //.
+proc*.
+outline {1} [1] { r <@ ROc.IdealAll.MainD(Red_ROM(A), ROc.IdealAll.RO).distinguish(); }.
+
++ inline; wp.
+  call (: ={servers, c_smap, s_smap, tested, kp_set, bad}(Game1, Red_ROM.AKE_O) /\ Game1.hm{1} = ROc.IdealAll.RO.m{2}); 
+    try sim />.
+
+  + proc; inline.
+    case ((x \in Game1.hm){1}).
+    - auto => />.
+    sp; seq 1 1: (#pre /\ tk{1} = r{2}); 1: by auto.
+    auto => />.
+
+  + proc; inline.
+    sp 2 2; match = => // sk.
+    match = => //.
+    seq 1 1: (#pre /\ ={kp}); 1: by auto.
+    sp 1 1; if => //.
+    sp. seq 1 1: (#pre /\ tk{1} = r0{2}); 1: by auto => />.
+    auto => />.
+
+  + proc; inline.
+    sp 1 1; match = => // st.
+    match = => // st' pt ir.
+    sp. seq 1 1: (#pre /\ tk{1} = r0{2}); 1: by auto.
+    auto => />.
+
+by call (ROSc.RO_split (Red_ROM(A))).
+qed.
+
+
 
 (* ------------------------------------------------------------------------------------------ *)
 (* Step 3: Moving sampling of the shared key. *)
 print ROSc.
 
-
+(* Clearing the key out of the state *)
 local op s_clear_k (s : pr_st_server instance_state) =
 match s with
 | Pending _ _ _ => s
@@ -221,11 +567,12 @@ match s with
 | Aborted _ _ _ => s
 end.
 
+(* Equivalence of partnering notions after keys are cleared *)
 local lemma c_eq_partners_ck tr sml smr: 
   (forall h, omap (fun (v: pr_st_server instance_state) => s_clear_k v) sml.[h] = smr.[h]) =>
 untested_partner_c tr sml = untested_partner_c tr smr.
 proof.
-move=> eqsm; rewrite /untested_partner_c.
+move=> eqsm @/untested_partner_c.
 have ->: get_partners_c tr sml = get_partners_c tr smr.
 + rewrite /get_partners_c; apply: fsetP=> x; rewrite !mem_fdom.
   rewrite !mem_filter !domE -eqsm.
@@ -240,7 +587,7 @@ local lemma s_eq_partners_ck tr sml smr:
   (forall h, omap (fun (v: pr_st_client instance_state) => c_clear_k v) sml.[h] = smr.[h]) =>
 untested_partner_s tr sml = untested_partner_s tr smr.
 proof.
-move=> eqsm; rewrite /untested_partner_s.
+move=> eqsm @/untested_partner_s.
 have ->: get_partners_s tr sml = get_partners_s tr smr.
 + rewrite /get_partners_s; apply: fsetP=> x; rewrite !mem_fdom.
   rewrite !mem_filter !domE -eqsm.
@@ -305,11 +652,9 @@ proc*.
 outline {1} [1] { r <@ ROSc.I2.MainD(Red_ROM2(A, ROSc.I1.RO), ROSc.I2.RO).distinguish(); }.
 
 + inline*; wp.
-  call (: ={hm, servers, kp_set, bad}(Red_ROM.AKE_O, Red_ROM2.AKE_O) /\ ={ROSc.I1.RO.m, ROSc.I2.RO.m}
+  call (: ={hm, servers, tested, kp_set, bad}(Red_ROM.AKE_O, Red_ROM2.AKE_O) /\ ={ROSc.I1.RO.m, ROSc.I2.RO.m}
           /\ (forall h, omap (fun v => c_clear_k v) Red_ROM.AKE_O.c_smap.[h]{1} = Red_ROM2.AKE_O.c_smap.[h]{2})
           /\ (forall h, omap (fun v => s_clear_k v) Red_ROM.AKE_O.s_smap.[h]{1} = Red_ROM2.AKE_O.s_smap.[h]{2})
-          /\ (forall i b pk1 pk2 sk pt ir, Red_ROM.AKE_O.c_smap{1}.[i] = Some (Pending (b, pk1, pk2, sk) pt ir)
-                => ir.`2 = false)
           /\ (forall i st pt k ir, Red_ROM.AKE_O.c_smap{1}.[i] = Some (Accepted st pt k ir)
                 => Red_ROM2.AKE_O.c_smap{2}.[i] = Some (Accepted st pt witness ir)
                    /\ ((oget pt.`2).`1 ^ st.`4, st.`2 ^ st.`4, st.`1, st.`3, (oget pt.`2).`1) \in ROSc.I2.RO.m{2}
@@ -344,7 +689,7 @@ outline {1} [1] { r <@ ROSc.I2.MainD(Red_ROM2(A, ROSc.I1.RO), ROSc.I2.RO).distin
     seq 1 1: (#pre /\ ={kp}); 1:by auto.
     sp 1 1; if => //.
     swap {1} ^r0<$ @ 1; swap {1} ^r3<$ @ 2.
-    swap {2} ^r0<$ @ 1; swap {2} ^r1<$ @ 2.
+    swap {2} ^r0<$ @ 1; swap {2} ^r1<$ @ 2. 
     seq  2  2: (#pre /\ ={r0} /\ r3{1} = r1{2}); 1: by auto=> />.
     sp 4 3; if {1} => //.
       + rcondt {1} ^if; 1: by auto => /#.
@@ -384,7 +729,7 @@ oget ROSc.I2.RO.m{2}.[m3{2}.`1 ^ sk_ce{2}, pk_b{2} ^ sk_ce{2}, b{2}, pk_ce{2}, m
     + auto=> /> &1 &2.
       case _: (Red_ROM.AKE_O.c_smap{1}.[i{2}])=> /> c_smap1_i.
       case _: (Red_ROM2.AKE_O.c_smap.[i]{2})=> /> c_smap2_i.
-      move=> c_clear s_clear inv1 inv2 inv3 eq_dom mem_ro.
+      move=> c_clear s_clear inv1 inv2 eq_dom mem_ro.
       move: c_smap2_i; rewrite -c_clear.
       rewrite c_smap1_i=> />. 
       smt(mem_set get_setE).
@@ -409,7 +754,7 @@ oget ROSc.I2.RO.m{2}.[m3{2}.`1 ^ sk_ce{2}, pk_b{2} ^ sk_ce{2}, b{2}, pk_ce{2}, m
     auto => /> &1 &2.
     case _: (Red_ROM.AKE_O.c_smap{1}.[i{2}])=> /> c_smap1_i.
     case _: (Red_ROM2.AKE_O.c_smap.[i]{2})=> /> c_smap2_i.
-    move=> c_clear s_clear inv1 inv2 inv3 eq_dom H k _. 
+    move=> c_clear s_clear inv1 inv2 eq_dom H k _. 
     smt(get_setE mem_set).
 
   - proc; inline.
@@ -425,7 +770,7 @@ oget ROSc.I2.RO.m{2}.[m3{2}.`1 ^ sk_ce{2}, pk_b{2} ^ sk_ce{2}, b{2}, pk_ce{2}, m
     auto => /> &1 &2.
     case _: (Red_ROM.AKE_O.s_smap{1}.[(b, j){2}])=> /> s_smap1_i.
     case _: (Red_ROM2.AKE_O.s_smap.[(b, j)]{2})=> /> s_smap2_i.
-    move=> c_clear s_clear inv1 inv2 inv3 eq_dom _ k _.
+    move=> c_clear s_clear inv1 inv2 eq_dom _ k _.
     smt(get_setE).
   
   - proc; inline.
@@ -433,9 +778,17 @@ oget ROSc.I2.RO.m{2}.[m3{2}.`1 ^ sk_ce{2}, pk_b{2} ^ sk_ce{2}, b{2}, pk_ce{2}, m
     move => stl str.
     match = => // kp.
     if => //.
-    + move => &1 &2 pre. print mem_set.
-      (* smt(c_eq_partners_ck). *)
-      admit. 
+    + move => /> &1 &2 hkp _ sstl sstr c_clear s_clear inv1 inv2 eq_dom.
+      split.
+      + move => + j - /(_ j). 
+        rewrite !domE -s_clear => />. search omap ("_.[_]").
+        case : (Red_ROM.AKE_O.s_smap.[b{2}, j]{1}) => />.
+        smt(s_eq_partners_ck). 
+      clear inv1 inv2.
+      move => + j - /(_ j). 
+      rewrite !domE -s_clear => />. search omap ("_.[_]").
+      case : (Red_ROM.AKE_O.s_smap.[b{2}, j]{1}) => />.
+      smt(s_eq_partners_ck).
     auto => />.
   
   - proc; inline.
@@ -466,7 +819,7 @@ oget ROSc.I2.RO.m{2}.[m3{2}.`1 ^ sk_ce{2}, pk_b{2} ^ sk_ce{2}, b{2}, pk_ce{2}, m
     smt(get_setE).
   
   - proc; inline.
-    sp; match => //.
+    sp; if => //. sp; match => //.
     + smt().
     + smt().
     move => stl str.
@@ -479,7 +832,7 @@ oget ROSc.I2.RO.m{2}.[m3{2}.`1 ^ sk_ce{2}, pk_b{2} ^ sk_ce{2}, b{2}, pk_ce{2}, m
     smt(get_setE).
 
   - proc; inline.
-    sp; match => //.
+    sp; if => //; sp; match => //.
     + smt().
     + smt().
     move => stl str.
@@ -494,8 +847,8 @@ oget ROSc.I2.RO.m{2}.[m3{2}.`1 ^ sk_ce{2}, pk_b{2} ^ sk_ce{2}, b{2}, pk_ce{2}, m
 have ll : forall (c : pkey * pkey * s_id * pkey * pkey), is_lossless dkey by move=> _; exact dkey_ll.
 rewrite equiv [{1} 1 (ROSc.I2.FullEager.RO_LRO (Red_ROM2(A, ROSc.I1.RO)) ll)].
 
-inline*; wp.
-call (: ={hm, servers, c_smap, s_smap, kp_set, bad}(Red_ROM2.AKE_O, Game2) /\ ROSc.I1.RO.m{1} = Game2.h1m{2} /\ ROSc.I2.RO.m{1} = Game2.h2m{2});
+inline; wp.
+call (: ={hm, servers, c_smap, s_smap, tested, kp_set, bad}(Red_ROM2.AKE_O, Game2) /\ ROSc.I1.RO.m{1} = Game2.h1m{2} /\ ROSc.I2.RO.m{1} = Game2.h2m{2});
  try sim />.
 
 - by proc; inline; auto => />.
@@ -526,13 +879,13 @@ call (: ={hm, servers, c_smap, s_smap, kp_set, bad}(Red_ROM2.AKE_O, Game2) /\ RO
   smt(get_setE mem_set).
 
 - proc; inline.
-  sp; match = => // st.
+  sp; if => //. sp; match = => // st.
   match = => // st' pt' k' ir'.
   if => //. auto => />.
   smt(get_setE mem_set).
 
 - proc; inline.
-  sp; match = => // st.
+  sp; if => //. sp; match = => // st.
   match = => // st' pt' k' ir'.
   if => //. auto => />.
   smt(get_setE mem_set).
@@ -541,297 +894,6 @@ auto => />.
 qed.
 
 
-(* ------------------------------------------------------------------------------------------ *)
-(* Step 2: Splitting the random oracle. *)
-local clone import DProd.ProdSampling with
-  type t1 <- tag,
-  type t2 <- key
-proof *.
-
-lemma Step2 &m: Pr[E_GAKE(Game1, A).run() @ &m : res] = Pr[ROc.IdealAll.MainD(Red_ROM(A), ROSc.RO_Pair(ROSc.I1.RO,ROSc.I2.RO)).distinguish() @ &m : res].
-proof.
-byequiv (: ={glob A, glob Red_ROM} ==> _)  => //.
-proc*.
-outline {1} [1] { r <@ ROc.IdealAll.MainD(Red_ROM(A), ROc.IdealAll.RO).distinguish(); }.
-
-+ inline; wp.
-  call (: ={servers, c_smap, s_smap, kp_set, bad}(Game1, Red_ROM.AKE_O) /\ Game1.hm{1} = ROc.IdealAll.RO.m{2}); 
-    try sim />.
-
-  + proc; inline.
-    case ((x \in Game1.hm){1}).
-    - auto => />.
-    sp; seq 1 1: (#pre /\ tk{1} = r{2}); 1: by auto.
-    auto => />.
-
-  + proc; inline.
-    sp 2 2; match = => // sk.
-    match = => //.
-    seq 1 1: (#pre /\ ={kp}); 1: by auto.
-    sp 1 1; if => //.
-    sp. seq 1 1: (#pre /\ tk{1} = r0{2}); 1: by auto => />.
-    auto => />.
-
-  + proc; inline.
-    sp 1 1; match = => // st.
-    match = => // st' pt ir.
-    sp. seq 1 1: (#pre /\ tk{1} = r0{2}); 1: by auto.
-    auto => />.
-
-by call (ROSc.RO_split (Red_ROM(A))).
-qed.
-
-
-(* ------------------------------------------------------------------------------------------ *)
-(* Step 0: Inlining everything. *)
-lemma Step0 &m :
-  Pr[E_GAKE(GAKE0(NTOR_S(RO), NTOR_C(RO), RO), A).run() @ &m : res] = Pr[E_GAKE(Game0, A).run() @ &m : res].
-proof. 
-byequiv => //.
-proc; inline*.
-call (: ={servers, c_smap, s_smap}(GAKEb, Game0) /\ RO.m{1} = Game0.hm{2}); try sim />.
-
-- proc; inline*; auto; if => //; auto => /#.
-
-- proc; inline*. 
-  sp; if => //.
-  sp; match = => // [|st]; 1:by auto.
-  by match = => // st' pt' ir'; auto.
-
-- proc; inline*.
-  sp; match = => // sk.
-  match = => //.
-  match Some {1} 4.
-  + by auto=> /> _ _ _ _; exists (b{m0}, sk, None).
-  match Some {1} ^match=> //; 1: by auto=> /> /#.
-  by auto => />.
-
-- proc; inline*; auto=> />.
-  sp; match = => //; 1: auto.
-  by match = => //; 1: auto.
-qed.
-
-(* ------------------------------------------------------------------------------------------ *)
-(* Step 1: Remove collisions in ephemeral and long-term keys. *)
-lemma Step1 &m: `| Pr[E_GAKE(Game0, A).run() @ &m : res] - Pr[E_GAKE(Game1, A).run() @ &m : res] | <= Pr[E_GAKE(Game0, A).run() @ &m : Game0.bad].
-proof.
-rewrite StdOrder.RealOrder.distrC.
-byequiv (: _ ==> _) : Game1.bad => //; first last.
-+ by rewrite eq_iff.
-symmetry; proc; inline*.
-call (: Game1.bad
-      , ={servers, c_smap, s_smap, kp_set, hm, bad}(Game0, Game1)
-      , ={bad}(Game0, Game1)) => //. 
-
-- exact A_ll.
-
-- by proc; auto.
-- move => &2 bad; proc; auto => />. 
-  by rewrite weight_dprod dkey_ll dtag_ll.
-- move => &1; proc; auto.
-  by rewrite weight_dprod dkey_ll dtag_ll.
-
-- proc.
-  if => //.
-  seq 1 1: (#pre /\ ={kp}); 1: by auto.
-  by sp 0 1; if{2}; auto => />.
-- move => &2 bad.
-  proc; if; auto.
-  rewrite dkp_ll //=. smt().
-- move => &1. 
-  proc; if => //. 
-  rcondf ^if; auto => />.
-  by rewrite dkp_ll.
-
-- proc; auto => />.
-- move => &2 bad.
-  proc; auto => />.
-- move => &1. 
-  proc; auto => />. 
-
-- proc.
-  sp; if => //.
-  sp; match = => //. 
-  + seq 1 1: (#pre /\ ={kp}); 1: by auto.
-    by sp 0 1; if{2}; auto => />.
-  move => st. 
-  match = => //.
-  move => st' pr' ir'.
-  auto => />.
-- move => &2 bad.
-  proc; sp; if => //; sp. 
-  match; auto => />.
-  + rewrite dkp_ll. smt().
-  by smt().
-- move => &1. 
-  proc; sp; if => //. 
-  sp; match; auto => />.
-  + by rewrite dkp_ll.
-  by smt().
-
-- proc; inline*.
-  sp; match = => //. 
-  move => sk.
-  match = => //.
-  + seq 1 1: (#pre /\ ={kp}); 1: by auto.
-  sp 0 1; if{2}.
-  + by auto => />. 
-  auto.
-- move => &2 bad.
-  proc; inline*; sp; match; auto => />.
-  match; auto => />.
-  rewrite dkp_ll weight_dprod dkey_ll dtag_ll. 
-  by smt().
-- move => &1. 
-  proc; sp; match; auto => />.
-  match; 2: by auto => />. 
-  rcondf ^if; 1: by auto => />. 
-  auto => />.
-  by rewrite dkp_ll.
-
-- sim />.
-- move => &2 bad.
-  proc; inline*.
-  sp; match; auto. 
-  match; auto => />.
-  by rewrite weight_dprod dkey_ll dtag_ll.
-- move => &1.
-  proc; inline*; auto => />.
-  sp; match; auto.
-  match; auto.
-  by rewrite weight_dprod dkey_ll dtag_ll.
-
-- sim />.
-- move => &2 bad.
-  proc; sp; match; 1: by auto. 
-  match; auto => />.
-- move => &1.
-  proc; sp; match; 1: by auto. 
-  match; auto => />.
-
-- sim />.
-- move => &2 bad.
-  proc; sp; match; 1: by auto. 
-  match; auto => />.
-- move => &1.
-  proc; sp; match; 1: by auto. 
-  match; auto => />.
-
-- sim />.
-- move => &2 bad.
-  proc; sp; match; 1: by auto. 
-  match; auto => />.
-- move => &1.
-  proc; sp; match; 1: by auto. 
-  match; auto => />.
-
-- sim />.
-- move => &2 bad.
-  proc; sp; match; 1: by auto. 
-  match; auto => />.
-- move => &1.
-  proc; sp; match; 1: by auto. 
-  match; auto => />.
-
-- sim />.
-- move => &2 bad.
-  proc; sp; match; 1: by auto. 
-  match; auto => />.
-- move => &1.
-  proc; sp; match; 1: by auto. 
-  match; auto => />.
-
-- sim />.
-- move => &2 bad.
-  proc; sp; match; 1: by auto. 
-  match; auto => />.
-- move => &1.
-  proc; sp; match; 1: by auto. 
-  match; auto => />.
-
-- sim />.
-- move => &2 bad.
-  proc; sp; match; 1: by auto. 
-  match; auto => />.
-- move => &1.
-  proc; sp; match; 1: by auto. 
-  match; auto => />.
-
-auto => />.
-move => rl rr al bl csl hml kpl ssl sl ar br csr hmr kpr ssr sr. 
-by case : (!br) => />.
-qed.
-
-
-(* ------------------------------------------------------------------------------------------ *)
-(* Step 1b: Bound the bad event. *)
-lemma Step1b &m: Pr[E_GAKE(Game0, A).run() @ &m : Game0.bad] <= ((q_is + q_m1 + q_m2) ^ 2)%r * mu1 dkp (mode dkp).
-proof.
-apply (StdOrder.RealOrder.ler_trans Pr[BB.Exp(BB.Sample, Red_Coll(A)).main() @ &m : ! uniq BB.Sample.l]); first last.
-+ apply (BB.pr_collision_q2 (Red_Coll(A))).
-  + move => S S_ll.
-    islossless.
-    apply (A_ll (Counter(Red_Coll_O_AKE(S)))); islossless.
-    + match; 1: auto; islossless.
-      match; auto.
-    + match; auto. 
-      by sp; match; auto; islossless.
-    + match => //.
-      by sp; match; auto; islossless.
-    + match => //; islossless.
-      by match; islossless.
-    + by match; 1: auto; match; islossless.
-    + by match; 1: auto; match; islossless.
-    + by match; 1: auto; match; islossless.
-    + by match; 1: auto; match; islossless.
-    + by match; 1: auto; match; islossless.
-    + by match; 1: auto; match; islossless.
-  proc; inline.
-  sp.
-  conseq (: _ ==> size BB.Sample.l <= Counter.cis + Counter.cm1 + Counter.cm2) (: Counter.cis = 0 /\ Counter.cm1 = 0 /\ Counter.cm2 = 0 ==> Counter.cis <= q_is /\ Counter.cm1 <= q_m1 /\ Counter.cm2 <= q_m2)=> //.
-  + smt().
-  + by call (A_bounded_qs (Red_Coll_O_AKE(BB.Sample))).
-  call (: size BB.Sample.l <= Counter.cis + Counter.cm1 + Counter.cm2) => //.
-  + by proc; auto.
-  + by proc; inline; sp; if => //; auto => /#.
-  + by proc; auto.
-  + proc; inline; sp; if => //; 2: auto => /#.
-    by sp; match; auto => /#.
-  + proc; inline; sp; match; 1: auto => /#.
-    case ((Red_Coll_O_AKE.s_smap.[b, j]) = None).
-    + by match None ^match; auto => /#.
-    by match Some ^match; auto => /#.
-  + by proc; inline; sp; match; 1: auto; match; auto => /#.
-  + by proc; sp; match; 1: auto; match; auto => /#.
-  + by proc; sp; match; 1: auto; match; auto => /#.
-  + by proc; sp; match; 1: auto; match; auto => /#.
-  + by proc; sp; match; 1: auto; match; auto => /#.
-  + by proc; sp; match; 1: auto; match; auto => /#.
-  + by proc; sp; match; 1: auto; match; auto => /#.
-  + by proc; sp; match; 1: auto; match; auto => /#.
-  auto => /#.
-byequiv => //.
-proc; inline.
-call (:
- ={hm, outs_h, servers, c_smap, s_smap, kp_set, bad, bad_ro}(Game0, Red_Coll_O_AKE(BB.Sample))
- /\ (Game0.bad{1} => !uniq BB.Sample.l{2})
- /\ (forall kp, kp \in Game0.kp_set{1} => kp \in BB.Sample.l{2})
-) => //; try sim />.
-+ proc; inline; sp 0 2; if => //; auto => />. 
-  smt(mem_set in_fsetU1).
-+ proc; inline; sp 2 4; if => //; auto.
-  sp; match = => // [|st].
-  + auto => />.
-    smt(mem_set in_fsetU1).
-  match = => // st' pt ir. 
-  auto => />.
-+ proc; inline; sp 2 4; match = => // [|st]; 1: auto.
-  match = => // [|st']; 2: auto.
-  auto => />.
-  smt(mem_set in_fsetU1).
-auto => />.
-smt(in_fset0).
-qed.
 
 
 end section.
